generating program with tests included

src/Tests/Test.thy
@@ -1,5 +1,5 @@
 theory Test
-imports Main "../SmallStep" "../Pretty"
+imports Main "../SmallStep" "../Pretty" "../GraphTest"
 begin
 
 abbreviation "aa \<equiv> ''a''"  abbreviation "bb \<equiv> ''b''" abbreviation "cc \<equiv> ''c''"
@@ -26,5 +26,109 @@ term remdups
 definition "execute_show vnames p \<equiv> case execute p of
   Some s \<Rightarrow> show_state (program.globals p @ (remdups (collect_locals (program.procs p))) @ vnames) s
   | None \<Rightarrow> show ''<Error>''"
+
+fun get_value_node :: "node list_graph \<Rightarrow> addr \<Rightarrow> val" where
+  "get_value_node graph addr = (case (lookup_node addr (nodesL graph)) of
+(* Node in memory doesn't exist, probably already deallocated, in this case, this
+  would be an error, there would be no program to test because it wouldn't have
+  been generated in the first place *)
+            None \<Rightarrow> NullVal |
+            Some node \<Rightarrow> (case (node.content node) of
+              Val i \<Rightarrow> I i |
+(* This would be an error, there would be no program to test because it wouldn't have
+  been generated in the first place *)
+              U \<Rightarrow> NullVal | 
+              P addr \<Rightarrow> A addr |
+(* This would be an error, there would be no program to test because it wouldn't have
+  been generated in the first place *)
+              InvalidP \<Rightarrow> NullVal))"
+
+fun is_addr :: "(nat \<times> val) \<Rightarrow> bool" where
+  "is_addr (_, (A _)) = True"
+| "is_addr (_, _) = False"
+
+lemma is_addr_addr[simp]:
+  assumes "is_addr (n, v)"
+  shows "\<exists>addr. v = A addr"
+  proof (cases v)
+    case NullVal
+      hence "is_addr (n, v) \<equiv> False" using is_addr_def by auto
+      hence "False" using `is_addr (n,v)` by blast
+      thus ?thesis by simp
+  next
+    case (I i)
+      hence "is_addr (n, v) \<equiv> False" using is_addr_def by auto
+      hence "False" using `is_addr (n,v)` by blast
+      thus ?thesis by simp
+  next
+    case (A addr)
+      thus ?thesis by simp
+qed
+
+(* n is how nested the actual value is, how many pointers must be followed in order to get to the value *)
+fun follow_object_graph :: "nat \<Rightarrow> addr \<Rightarrow> node list_graph \<Rightarrow> (nat \<times> val)" where
+  "follow_object_graph n addr graph = (while
+    (is_addr)
+    (\<lambda>(n, A addr) \<Rightarrow> (n+1, get_value_node graph addr))
+    (n, get_value_node graph addr))"
+
+value "shows_graph memory_graph ''''"
+definition "test \<equiv> (construct_graph [None, Some [(Some (A (2,0))), Some (A (2,1))], Some [(Some (A (1,1))), Some (I 4), None]])"
+value "follow_object_graph 0 (1,0) test"
+
+fun follow_pointer :: "nat \<Rightarrow> exp \<Rightarrow> exp" where
+  "follow_pointer 0 e = e"
+| "follow_pointer n e = follow_pointer (n-1) (Deref e)"
+
+fun generate_test :: "exp \<Rightarrow> val \<Rightarrow> node list_graph \<Rightarrow> com" where
+  "generate_test x value graph =
+      (case value of 
+        NullVal \<Rightarrow>
+          IF (Eq x (Null))
+          THEN
+            (''num_tests'' ::= (Plus (V ''num_tests'') (Const 1));;
+            ''passed'' ::= (Plus (V ''passed'') (Const 1)))
+          ELSE
+            (''num_tests'' ::= (Plus (V ''num_tests'') (Const 1));;
+            ''failed'' ::= (Plus (V ''failed'') (Const 1))) |
+        I i \<Rightarrow>
+          IF (Eq x (Const i))
+          THEN
+            (''num_tests'' ::= (Plus (V ''num_tests'') (Const 1));;
+            ''passed'' ::= (Plus (V ''passed'') (Const 1)))
+          ELSE
+            (''num_tests'' ::= (Plus (V ''num_tests'') (Const 1));;
+            ''failed'' ::= (Plus (V ''failed'') (Const 1))) |
+        A addr \<Rightarrow>
+          let
+            (n, v) = follow_object_graph 0 addr graph;
+            lval = follow_pointer n (Deref x)
+          in
+            (case v of
+              (I i) \<Rightarrow>
+                IF (Eq lval (Const i))
+                THEN
+                  (''num_tests'' ::= (Plus (V ''num_tests'') (Const 1));;
+                  ''passed'' ::= (Plus (V ''passed'') (Const 1)))
+                ELSE
+                  (''num_tests'' ::= (Plus (V ''num_tests'') (Const 1));;
+                  ''failed'' ::= (Plus (V ''failed'') (Const 1))) |
+              _ \<Rightarrow> SKIP (* Should never happen *)
+            )
+      )"
+
+(* vname list and val list must have the same length *)
+fun generate_tests :: "exp list \<Rightarrow> val list \<Rightarrow> node list_graph \<Rightarrow> com" where
+  "generate_tests [] [] graph = SKIP"
+| "generate_tests (x#xs) (y#ys) graph = generate_test x y graph;; generate_tests xs ys graph"
+
+(* vname list and val list must have the same length *)
+fun generate_test_function :: "exp list \<Rightarrow> val list \<Rightarrow> node list_graph \<Rightarrow> fun_decl" where
+  "generate_test_function x y graph= 
+    \<lparr> fun_decl.name = ''test'',
+      fun_decl.params = [],
+      fun_decl.locals = [],
+      fun_decl.body = generate_tests x y graph
+    \<rparr>"
 
 end
